src/Prelude.thy
@@ -1,9 +1,20 @@
-theory Prelude imports Main begin
+theory Prelude imports Main Util begin
 
-(* FIXME move to lib *)
 definition from_to :: "nat \<Rightarrow> nat \<Rightarrow> nat list" where
 "from_to x y = upt x (Suc y)"
 
 
+definition maps_as_map :: "('a,'b) map set \<Rightarrow> ('a,'b) map \<Rightarrow> bool" where
+"maps_as_map ms m = (
+(! a b. (m a = Some b) = (? m' : ms. m' a = Some b)) &
+(! a. (m a = None) = (! m' : ms. m' a = None))
+)"
+
+definition merge_maps :: "('a,'b) map set \<Rightarrow> ('a,'b) map" where
+"merge_maps ms = (SOME m. maps_as_map ms m)"
+
+lemma "maps_as_map ms (merge_maps ms)"
+  apply(force intro:FIXME)
+  done
 
 end
